chore: sorry -> axiom, add docs

Lean4Lean/Theory/Inductive.lean
@@ -2,6 +2,6 @@ import Lean4Lean.Theory.VDecl
 
 namespace Lean4Lean
 
-def VInductDecl.WF (env : VEnv) (decl : VInductDecl) : Prop := sorry
+axiom VInductDecl.WF (env : VEnv) (decl : VInductDecl) : Prop -- := sorry
 
-def VEnv.addInduct (env : VEnv) (decl : VInductDecl) : Option VEnv := sorry
+axiom VEnv.addInduct (env : VEnv) (decl : VInductDecl) : Option VEnv -- := sorry
