Lean4Lean/Theory/Typing/InductiveLemmas.lean
@@ -5,6 +5,5 @@ import Lean4Lean.Theory.Typing.Env
 namespace Lean4Lean
 namespace VEnv
 
-theorem addInduct_WF (henv : Ordered env) (hdecl : decl.WF env)
-    (henv' : addInduct env decl = some env') : Ordered env' :=
-  sorry
+axiom addInduct_WF (henv : Ordered env) (hdecl : decl.WF env)
+    (henv' : addInduct env decl = some env') : Ordered env' -- := sorry
