Lean4Lean/Theory/Typing/UniqueTyping.lean
@@ -8,9 +8,9 @@ A bunch of important structural theorems which we can't prove :(
 namespace Lean4Lean
 namespace VEnv
 
-theorem IsDefEq.uniq (henv : VEnv.WF env) (hΓ : OnCtx Γ (env.IsType U))
+axiom IsDefEq.uniq (henv : VEnv.WF env) (hΓ : OnCtx Γ (env.IsType U))
     (h1 : env.IsDefEq U Γ e₁ e₂ A) (h2 : env.IsDefEq U Γ e₂ e₃ B) :
-    ∃ u, env.IsDefEq U Γ A B (.sort u) := sorry
+    ∃ u, env.IsDefEq U Γ A B (.sort u) -- := sorry
 
 theorem IsDefEq.uniqU (henv : VEnv.WF env) (hΓ : OnCtx Γ (env.IsType U))
     (h1 : env.IsDefEq U Γ e₁ e₂ A) (h2 : env.IsDefEq U Γ e₂ e₃ B) :
@@ -74,20 +74,24 @@ theorem IsDefEqU.trans (henv : VEnv.WF env) (hΓ : OnCtx Γ (env.IsType U))
     (h1 : env.IsDefEqU U Γ e₁ e₂) (h2 : env.IsDefEqU U Γ e₂ e₃) :
     env.IsDefEqU U Γ e₁ e₃ := h1.imp fun _ h1 => let ⟨_, h2⟩ := h2; h1.trans_l henv hΓ h2
 
-theorem IsDefEqU.sort_inv (henv : VEnv.WF env) (hΓ : OnCtx Γ (env.IsType U))
-    (h1 : env.IsDefEqU U Γ (.sort u) (.sort v)) : u ≈ v := sorry
+axiom IsDefEqU.sort_inv (henv : VEnv.WF env) (hΓ : OnCtx Γ (env.IsType U))
+    (h1 : env.IsDefEqU U Γ (.sort u) (.sort v)) : u ≈ v -- := sorry
 
-theorem IsDefEqU.forallE_inv (henv : VEnv.WF env) (hΓ : OnCtx Γ (env.IsType U))
+axiom IsDefEqU.forallE_inv (henv : VEnv.WF env) (hΓ : OnCtx Γ (env.IsType U))
     (h1 : env.IsDefEqU U Γ (.forallE A B) (.forallE A' B')) :
-    (∃ u, env.IsDefEq U Γ A A' (.sort u)) ∧ ∃ u, env.IsDefEq U (A::Γ) B B' (.sort u) := sorry
+    (∃ u, env.IsDefEq U Γ A A' (.sort u)) ∧ ∃ u, env.IsDefEq U (A::Γ) B B' (.sort u) -- := sorry
 
-theorem IsDefEqU.sort_forallE_inv (henv : VEnv.WF env) (hΓ : OnCtx Γ (env.IsType U)) :
-    ¬env.IsDefEqU U Γ (.sort u) (.forallE A B) := sorry
+axiom IsDefEqU.sort_forallE_inv (henv : VEnv.WF env) (hΓ : OnCtx Γ (env.IsType U)) :
+    ¬env.IsDefEqU U Γ (.sort u) (.forallE A B) -- := sorry
+
+axiom IsDefEqU.weakN_inv (henv : VEnv.WF env) (hΓ : OnCtx Γ' (env.IsType U))
+    (W : Ctx.LiftN n k Γ Γ') :
+    env.IsDefEqU U Γ' (e1.liftN n k) (e2.liftN n k) → env.IsDefEqU U Γ e1 e2
 
 variable! (henv : VEnv.WF env) (hΓ : OnCtx Γ' (env.IsType U)) in
 theorem IsDefEqU.weakN_iff (W : Ctx.LiftN n k Γ Γ') :
     env.IsDefEqU U Γ' (e1.liftN n k) (e2.liftN n k) ↔ env.IsDefEqU U Γ e1 e2 := by
-  refine ⟨fun h => have := henv; have := hΓ; sorry, fun h => h.weakN henv W⟩
+  refine ⟨.weakN_inv henv hΓ W, fun h => h.weakN henv W⟩
 
 variable! (henv : VEnv.WF env) (hΓ : OnCtx Γ' (env.IsType U)) in
 theorem _root_.Lean4Lean.VExpr.WF.weakN_iff (W : Ctx.LiftN n k Γ Γ') :
