Lean4Lean/Verify/Level.lean
@@ -154,8 +154,8 @@ open private substParams.go from Lean.Level in
 theorem substParams_id {u : Level} :
     substParams' .param false u = u := by induction u <;> simp_all [substParams']
 
-theorem isEquiv'_wf (h : isEquiv' u v)
-    (hu : VLevel.ofLevel ls u = some u') (hv : VLevel.ofLevel ls v = some v') : u' ≈ v' := sorry
+axiom isEquiv'_wf (h : isEquiv' u v)
+    (hu : VLevel.ofLevel ls u = some u') (hv : VLevel.ofLevel ls v = some v') : u' ≈ v' -- := sorry
 
 theorem isEquivList_wf (H : Level.isEquivList us vs) :
     List.mapM (VLevel.ofLevel Us) us = some us' →
