Lean4Lean/Verify/TypeChecker/IsDefEq.lean
@@ -221,9 +221,9 @@ theorem tryEtaExpansion.WF {c : VContext} {s : VState}
   split <;> [exact .pure fun _ => h rfl; skip]
   exact (tryEtaExpansionCore.WF he₂ he₁).mono fun _ _ _ h hb => (h hb).symm
 
-theorem tryEtaStructCore.WF {c : VContext} {s : VState}
+axiom tryEtaStructCore.WF {c : VContext} {s : VState}
     (he₁ : c.TrExprS e₁ e₁') (he₂ : c.TrExprS e₂ e₂') :
-    RecM.WF c s (tryEtaStructCore e₁ e₂) fun b _ => b → c.IsDefEqU e₁' e₂' := sorry
+    RecM.WF c s (tryEtaStructCore e₁ e₂) fun b _ => b → c.IsDefEqU e₁' e₂' -- := sorry
 
 theorem tryEtaStruct.WF {c : VContext} {s : VState}
     (he₁ : c.TrExprS e₁ e₁') (he₂ : c.TrExprS e₂ e₂') :
@@ -485,9 +485,9 @@ theorem tryStringLitExpansion.WF {c : VContext} {s : VState}
   split <;> [skip; exact .pure h]
   exact (tryStringLitExpansionCore.WF he₂ he₁).mono fun _ _ _ h hb => (h hb).symm
 
-theorem isDefEqUnitLike.WF {c : VContext} {s : VState}
+axiom isDefEqUnitLike.WF {c : VContext} {s : VState}
     (he₁ : c.TrExprS e₁ e₁') (he₂ : c.TrExprS e₂ e₂') :
-    RecM.WF c s (isDefEqUnitLike e₁ e₂) fun b _ => b = .true → c.IsDefEqU e₁' e₂' := sorry
+    RecM.WF c s (isDefEqUnitLike e₁ e₂) fun b _ => b = .true → c.IsDefEqU e₁' e₂' -- := sorry
 
 theorem isDefEqCore'.WF {c : VContext} {s : VState}
     (he₁ : c.TrExprS e₁ e₁') (he₂ : c.TrExprS e₂ e₂') :
