Lean4Lean/Verify/Typing/Lemmas.lean
@@ -546,8 +546,8 @@ inductive SortList : VLCtx → List VLevel → Prop
 
 end VLCtx
 
-theorem TrProj.weak' (W : Ctx.Lift' n Γ Γ')
-    (H : TrProj Γ s i e e') : TrProj Γ' s i (e.lift' n) (e'.lift' n) := sorry
+axiom TrProj.weak' (W : Ctx.Lift' n Γ Γ')
+    (H : TrProj Γ s i e e') : TrProj Γ' s i (e.lift' n) (e'.lift' n) -- := sorry
 
 theorem TrProj.weakN (W : Ctx.LiftN n k Γ Γ')
     (H : TrProj Γ s i e e') : TrProj Γ' s i (e.liftN n k) (e'.liftN n k) := by
@@ -627,12 +627,12 @@ theorem HasType.skips (W : Ctx.LiftN n k Γ Γ')
     (h1 : env.HasType U Γ' e A) (h2 : e.Skips n k) : ∃ B, env.HasType U Γ' e B ∧ B.Skips n k :=
   IsDefEq.skips henv hΓ' W h1 h2 h2
 
-theorem TrProj.weak'_inv (henv : VEnv.WF env) (hΓ' : OnCtx Γ' (env.IsType U))
-    (W : Ctx.Lift' l Γ Γ') : TrProj Γ' s i (e.lift' l) e' → ∃ e', TrProj Γ s i e e' := sorry
+axiom TrProj.weak'_inv (henv : VEnv.WF env) (hΓ' : OnCtx Γ' (env.IsType U))
+    (W : Ctx.Lift' l Γ Γ') : TrProj Γ' s i (e.lift' l) e' → ∃ e', TrProj Γ s i e e' -- := sorry
 
-theorem TrProj.defeqDFC (henv : VEnv.WF env) (hΓ : env.IsDefEqCtx U [] Γ₁ Γ₂)
+axiom TrProj.defeqDFC (henv : VEnv.WF env) (hΓ : env.IsDefEqCtx U [] Γ₁ Γ₂)
     (he : env.IsDefEqU U Γ₁ e₁ e₂) (H : TrProj Γ₁ s i e₁ e') :
-    ∃ e', TrProj Γ₂ s i e₂ e' := sorry
+    ∃ e', TrProj Γ₂ s i e₂ e' -- := sorry
 
 variable! {env env' : VEnv} (henv : env ≤ env') in
 theorem TrExprS.mono (H : TrExprS env Us Δ e e') : TrExprS env' Us Δ e e' := by
@@ -793,7 +793,7 @@ theorem TrExpr.fvarsIn (H : TrExpr env Us Δ e e') : FVarsIn (· ∈ Δ.fvars) e
 theorem TrExpr.fvarsList (H : TrExpr env Us Δ e e') : e.fvarsList ⊆ Δ.fvars :=
   (fvarsIn_iff.1 H.fvarsIn).1
 
-theorem TrProj.wf (H1 : TrProj Δ s i e e') (H2 : VExpr.WF env U Γ e) : VExpr.WF env U Γ e' := sorry
+axiom TrProj.wf (H1 : TrProj Δ s i e e') (H2 : VExpr.WF env U Γ e) : VExpr.WF env U Γ e' -- := sorry
 
 theorem TrExpr.wf (H : TrExpr env Us Δ e e') : VExpr.WF env Us.length Δ.toCtx e' :=
   let ⟨_, _, _, H⟩ := H; ⟨_, H.hasType.2⟩
@@ -835,10 +835,10 @@ theorem TrExpr.app (henv : VEnv.WF env) (hΔ : OnCtx Δ.toCtx (env.IsType Us.len
   have h4 := h4.of_r henv hΔ h2
   ⟨_, .app h3.hasType.1 h4.hasType.1 s3 s4, _, h3.appDF h4⟩
 
-variable! (henv : VEnv.WF env) (hΓ : IsDefEqCtx env U [] Γ₁ Γ₂) in
-theorem TrProj.uniq (H1 : TrProj Γ₁ s₁ i e₁ e₁') (H2 : TrProj Γ₂ s₂ i e₂ e₂')
+axiom TrProj.uniq (henv : VEnv.WF env) (hΓ : IsDefEqCtx env U [] Γ₁ Γ₂)
+    (H1 : TrProj Γ₁ s₁ i e₁ e₁') (H2 : TrProj Γ₂ s₂ i e₂ e₂')
     (H : env.IsDefEqU U Γ₁ e₁ e₂) :
-    env.IsDefEqU U Γ₁ e₁' e₂' := sorry
+    env.IsDefEqU U Γ₁ e₁' e₂' -- := sorry
 
 variable! (henv : VEnv.WF env) {Us : List Name} (hΔ : VLCtx.IsDefEq env Us.length Δ₁ Δ₂) in
 theorem TrExprS.uniq (H1 : TrExprS env Us Δ₁ e e₁) (H2 : TrExprS env Us Δ₂ e e₂) :
@@ -1138,8 +1138,8 @@ theorem TrExprS.instN_var (W : VLCtx.InstN Δ₀ e₀' A₀ dk k Δ₁ Δ) (H : 
         refine ⟨_, _, h, ?_, rfl⟩
         cases d <;> simp [VLocalDecl.depth, VLocalDecl.inst, VExpr.lift_instN_lo]
 
-theorem TrProj.instN (W : Ctx.InstN Γ₀ e₀ A₀ k Γ₁ Γ)
-    (H : TrProj Γ₁ s i e e') : TrProj Γ s i (e.inst e₀ k) (e'.inst e₀ k) := sorry
+axiom TrProj.instN (W : Ctx.InstN Γ₀ e₀ A₀ k Γ₁ Γ)
+    (H : TrProj Γ₁ s i e e') : TrProj Γ s i (e.inst e₀ k) (e'.inst e₀ k) -- := sorry
 
 variable! (henv : Ordered env) (h₀ : TrExprS env Us Δ₀ e₀ e₀')
   (t₀ : env.HasType Us.length Δ₀.toCtx e₀' A₀) in
@@ -1393,9 +1393,8 @@ theorem ofLevel_mkLevelIMax'
   · simp_all; exact VLevel.imax_self.symm
   simp [VLevel.ofLevel]; exact ⟨_, ⟨_, h1, _, h2, rfl⟩, rfl⟩
 
-variable! {ls : List VLevel} (hls : ∀ l ∈ ls, l.WF U') in
-theorem TrProj.instL (H : TrProj Γ s i e e') :
-    TrProj (Γ.map (VExpr.instL ls)) s i (e.instL ls) (e'.instL ls) := sorry
+axiom TrProj.instL {ls : List VLevel} (hls : ∀ l ∈ ls, l.WF U') (H : TrProj Γ s i e e') :
+    TrProj (Γ.map (VExpr.instL ls)) s i (e.instL ls) (e'.instL ls) -- := sorry
 
 section
 
