axioms.md
@@ -1,0 +1,109 @@
+# Axioms used in the main theorem
+
+Here is a complete listing and breakdown of the axioms used in
+[`Lean4Lean.TypeChecker.checkType.WF`](Lean4Lean/Verify/TypeChecker.lean) and friends:
+
+## • Lean builtin axioms
+
+These are normal in all Lean projects.
+
+* `propext`
+* `Classical.choice`
+* `Quot.sound`
+
+## • Axioms from [Axioms.lean](Lean4Lean/Verify/Axioms.lean)
+
+This file contains axioms which allow us to reason about the behavior of opaque
+functions. See [Axioms.lean](Lean4Lean/Verify/Axioms.lean) for more details about
+each axiom. This is the main coordination point for adapting to changes to Lean core.
+We use axioms deliberately here, rather than reimplementing verified versions of the
+functions (which can be done in many cases, and in fact most of these axioms assert
+that a function from core is equal to a simpler executable spec function), because
+a we want to ensure that we use the same function as the upstream kernel where possible.
+
+* `Lean.PersistentArray.toList'_push`
+* `Lean.PersistentHashMap.WF.toList'_insert`
+* `Lean.PersistentHashMap.WF.find?_eq`
+* `Lean.PersistentHashMap.findAux_isSome`
+* `Lean.Expr.mkAppRangeAux.eq_def`
+* `Lean.Substring.beq_refl`
+* `Lean.Syntax.structEq_eq`
+* `Lean.Level.hasParam_eq`
+* `Lean.Level.hasMVar_eq`
+* `Lean.Level.instLawfulBEqLevel`
+* `Lean.Expr.hasLevelParam_eq`
+* `Lean.Expr.looseBVarRange_eq`
+* `Lean.Expr.replace_eq`
+* `Lean.Expr.lowerLooseBVars_eq`
+* `Lean.Expr.instantiate1_eq`
+* `Lean.Expr.instantiate_eq`
+* `Lean.Expr.instantiateRev_eq`
+* `Lean.Expr.instantiateRange_eq`
+* `Lean.Expr.instantiateRevRange_eq`
+* `Lean.Expr.abstract_eq`
+* `Lean.Expr.abstractRange_eq`
+* `Lean.Expr.hasLooseBVar_eq`
+* `Lean.Expr.eqv_eq`
+
+## • Axioms about [ptrEq](Lean4Lean/PtrEq.lean)
+
+See [PtrEq.lean](Lean4Lean/PtrEq.lean). Pointer equality does not behave like a
+regular function, so we have to be careful with its use, but it is an important
+part of the kernel. We only care about one property, which is that if two objects
+are pointer-equal then they are propositionally equal, but while this is true for
+`ptrEq` generic over all types, the function itself is unsafe so we can't assume it
+outright. Even this form is questionable, but to mitigate possible issues with pointer identity of closures (function types), we specialize to `Expr` and `ConstantInfo`.
+
+* `Lean4Lean.ptrEqExpr_eq`
+* `Lean4Lean.ptrEqConstantInfo_eq`
+
+## • Sorries related to inductive types
+
+Currently inductive types are not modeled in the theory, so the parts of the kernel that deal with inductive types are sorried. (The "(sorry)" in these entries below mean
+that these are not real axioms, they can be proved in the future but are converted to axioms for ease of tracking.)
+
+* `Lean4Lean.VInductDecl.WF` (sorry)
+* `Lean4Lean.VEnv.addInduct` (sorry)
+* `Lean4Lean.VEnv.addInduct_WF` (sorry)
+
+The type checker functions which manipulate inductive types are not proved for the same reason.
+
+* `Lean4Lean.TypeChecker.Inner.isDefEqUnitLike.WF` (sorry)
+* `Lean4Lean.TypeChecker.Inner.reduceRecursor.WF` (sorry)
+* `Lean4Lean.TypeChecker.Inner.tryEtaStructCore.WF` (sorry)
+
+## • Sorries related to [TrProj](Lean4Lean/Verify/Typing/Expr.lean)
+
+Continuation of the above. Projections expand to a recursor application, so this also requires details of structures (which are a kind of inductive type). These axioms correspond essentially to the `proj` case of each main theorem about `TrExprS`.
+
+* `Lean4Lean.TrProj` (sorry)
+* `Lean4Lean.TrProj.defeqDFC` (sorry)
+* `Lean4Lean.TrProj.instL` (sorry)
+* `Lean4Lean.TrProj.instN` (sorry)
+* `Lean4Lean.TrProj.uniq` (sorry)
+* `Lean4Lean.TrProj.weak'` (sorry)
+* `Lean4Lean.TrProj.weak'_inv` (sorry)
+* `Lean4Lean.TrProj.wf` (sorry)
+
+The typechecker functions which manipulate projections are not proved for the same reason.
+
+* `Lean4Lean.TypeChecker.Inner.inferProj.WF` (sorry)
+* `Lean4Lean.TypeChecker.Inner.reduceProj.WF` (sorry)
+
+## • Sorries related to [unique typing](Lean4Lean/Theory/Typing/UniqueTyping.lean)
+
+This is the main conjecture discussed in the paper.
+
+* `Lean4Lean.VEnv.IsDefEq.uniq` (sorry)
+* `Lean4Lean.VEnv.IsDefEqU.forallE_inv` (sorry)
+* `Lean4Lean.VEnv.IsDefEqU.weakN_inv` (sorry)
+
+## • Sorries related to the new [`isEquiv'`](Lean4Lean/Level.lean)
+
+This relates to an experiment to replace the `isEquiv` function with a version `isEquiv'`
+which should be a complete normalization algorithm for level expressions. It is
+significantly more complex, however, and it hasn't been proved correct yet.
+It would be nice to prove it complete too, although in general completeness is
+not a goal of the typechecker.
+
+* `Lean.Level.isEquiv'_wf` (sorry)
